freest/test/prog/Invalid/RefinedSessions/InvalidReturnTypeOnSubtract/InvalidReturnTypeOnSubtract.fst
@@ -2,9 +2,9 @@ module InvalidReturnTypeOnSubtract where
 
 type BiggerThanTwo, BiggerThanFive, Negative : *T
 
-BiggerThanTwo  = {x: Int | x >= 2}
-BiggerThanFive = {y: Int | y >= 5}
-Negative       = {z: Int | z < 0}
+type BiggerThanTwo  = {x: Int | x >= 2}
+type BiggerThanFive = {y: Int | y >= 5}
+type Negative       = {z: Int | z < 0}
 
 specialSubtract : BiggerThanTwo -> BiggerThanFive -> Negative
 specialSubtract x y = x - y
