freest/test/prog/Valid/RefinedSessions/PolarIntTree/PolarIntTree.fst
@@ -1,21 +1,23 @@
 module InvalidIntInDataType where
 
 type PositiveInt, NegativeInt : *T
-type PolarTree : *T -> *T
+type PolarTree : *T -> *T -> *T
 
 type PositiveInt = {x: Int | x >= 0}
 type NegativeInt = {y: Int | y <= 0}
 
 -- Left of each node has type a and right has type b
-data PolarTree (a b : *T) =
+data PolarTree a b =
     Leaf
-  | Node (PolarTree @a @b) a (PolarTree @b @a)
+  | Node (PolarTree a b) a (PolarTree b a)
 
-buildPolarIntTree : PolarTree @PositiveInt @NegativeInt
-buildPolarIntTree = Node left 0 right
+buildPolarIntTree : PolarTree PositiveInt NegativeInt
+buildPolarIntTree = Node @PositiveInt @NegativeInt left 0 right
   where
-    left = Node (Node Leaf 2 Leaf) 1 (Node (Node Leaf 3 Leaf) -2 Leaf)
-    right = Node Leaf -1 Leaf
+    leftLeft = Node @PositiveInt @NegativeInt Leaf 2 Leaf
+    leftRight = Node @PositiveInt @NegativeInt (Node @PositiveInt @NegativeInt Leaf 3 Leaf) -2 Leaf
+    left = Node @PositiveInt @NegativeInt leftLeft 1 leftRight
+    right = Node @PositiveInt @NegativeInt Leaf -1 Leaf
 
 main : ()
-main = buildPolarIntTree;
+main = buildPolarIntTree; ()
