freest/test/prog/Valid/RefinedSessions/Sum/Sum.fst
@@ -2,9 +2,9 @@ module Sum where
 
 type BiggerThanTwo, BiggerThanFive, BiggerThanSeven : *T
 
-BiggerThanTwo   = {x: Int | x >= 2}
-BiggerThanFive  = {y: Int | y >= 5}
-BiggerThanSeven = {z: Int | z >= 7}
+type BiggerThanTwo   = {x: Int | x >= 2}
+type BiggerThanFive  = {y: Int | y >= 5}
+type BiggerThanSeven = {z: Int | z >= 7}
 
 specialSum : BiggerThanTwo -> BiggerThanFive -> BiggerThanSeven
 specialSum x y = x + y
